theories/coneris/lib/hocap.v
@@ -30,14 +30,14 @@ Section lemmas.
     - by eauto with iFrame.
   Qed.
 
-  Lemma hocap_error_agree γ b c :
+  Lemma hocap_error_agree γ (b c:R) :
     (●↯ b @ γ) -∗ (◯↯ c @ γ) -∗ ⌜ b = c ⌝.
   Proof.
     iIntros "[% [<- Hγ●]] [% [<-Hγ◯]]".
     by iCombine "Hγ● Hγ◯" gives %<-%excl_auth_agree_L.
   Qed.
 
-  Lemma hocap_error_update γ (b':nonnegreal) b c :
+  Lemma hocap_error_update γ (b':nonnegreal) (b c:R) :
     (●↯ b @ γ) -∗ (◯↯ c @ γ) ==∗ (●↯ b' @ γ) ∗ (◯↯ b' @ γ).
   Proof.
     iIntros "[% [<- Hγ●]] [% [<-Hγ◯]]".
@@ -61,16 +61,19 @@ Section HOCAP.
     ↑hocap_error_nroot ⊆ E ->
     (∀ (ε:nonnegreal), SeriesC (λ n, (1 / (S N)) * nonneg (ε2 ε n))%R <= (nonneg ε))%R →
     {{{ error_inv γ∗
-        (∀ (ε:nonnegreal) (n : fin (S N)), P ∗ ●↯ ε @ γ ={E∖↑hocap_error_nroot}=∗ ●↯ (ε2 ε n) @ γ ∗ Q (n) ) ∗
+        (∀ (ε:nonnegreal) (n : fin (S N)), P ∗ ●↯ ε @ γ ={E∖↑hocap_error_nroot}=∗
+                                           (●↯ (ε2 ε n) @ γ ∗ (⌜(1<=ε2 ε n)%R⌝ ∨ Q (n))) ) ∗
         P }}} rand #z @ E {{{ n, RET #n; Q (n)}}}.
   Proof.
     iIntros (-> Hsubset Hineq) "%Φ [#Hinv [Hchange HP]] HΦ".
     iInv "Hinv" as ">(%ε & Hε & Hauth)" "Hclose".
     wp_apply (wp_couple_rand_adv_comp1' with "[$]"); first apply Hineq.
     iIntros (n) "Hε".
-    iMod ("Hchange" $! _ n with "[$]") as "[Hauth HQ]".
-    iMod ("Hclose" with "[Hauth Hε]") as "_"; first iFrame.
-    by iApply "HΦ".
+    iMod ("Hchange" $! _ n with "[$]") as "[Hauth [%|HQ]]"; last first.
+    { iMod ("Hclose" with "[Hauth Hε]") as "_"; first iFrame.
+      by iApply "HΦ". }
+    iExFalso.
+    by iApply (ec_contradict with "[$]").
   Qed.
 
   Lemma wp_hocap_flip_adv_comp E
@@ -79,7 +82,7 @@ Section HOCAP.
     ↑hocap_error_nroot ⊆ E ->
     (∀ (ε:nonnegreal),  ((nonneg (ε2 ε true) + nonneg (ε2 ε false))/2 <= (nonneg ε))%R) →
     {{{ error_inv γ∗
-        □(∀ (ε:nonnegreal) (b : bool), P ∗ ●↯ ε @ γ ={E∖↑hocap_error_nroot}=∗ ●↯ (ε2 ε b) @ γ ∗ Q (b) ) ∗
+        □(∀ (ε:nonnegreal) (b : bool), P ∗ ●↯ ε @ γ ={E∖↑hocap_error_nroot}=∗ ●↯ (ε2 ε b) @ γ ∗ (⌜(1<=ε2 ε b)%R⌝ ∨ Q (b)) ) ∗
         P }}} flip @ E {{{ (b:bool), RET #b; Q (b)}}}.
   Proof.
     iIntros (Hsubset Hineq) "%Φ [#Hinv [#Hchange HP]] HΦ".
@@ -89,9 +92,8 @@ Section HOCAP.
     - intros ε. rewrite SeriesC_finite_foldr; simpl. specialize (Hineq ε). lra.
     - iFrame. iSplitR; first iExact "Hinv".
       iIntros (ε n) "H".
-      iMod ("Hchange" with "[$]") as "[Hε HQ]".
-      iModIntro. iSplitL "Hε"; last done.
-      by case_match.
+      iMod ("Hchange" $! _ (fin_to_nat n =? 1%nat)with "[$]") as "[Hε HQ]".
+      iModIntro. iSplitL "Hε"; by case_match. 
     - iIntros.
       wp_apply (conversion.wp_int_to_bool); first done.
       iIntros "_".
